Fix up specs enough to re-prove CREATE

src/Dafny/examples/fs/cursor.dfy
@@ -17,10 +17,15 @@ module FileCursor {
     const fs: TypedFilesys
 
     var off: uint64
-    var bs: Bytes?
+    var bs: Bytes
+    var valid?: bool
 
     // this doesn't include fs.Repr and i.Repr; we list those explicitly
-    var Repr: set<object>
+    function Repr(): set<object>
+      reads this
+    {
+      {this, bs}
+    }
 
     ghost const ReprFs: set<object> := fs.Repr + i.Repr
 
@@ -31,19 +36,12 @@ module FileCursor {
       && |fs.data[ino]| % 4096 == 0
       && off % 4096 == 0
       && bs !in i.Repr
-      && (bs != null ==> off as nat + 4096 <= |fs.data[ino]|)
-    }
-
-    predicate ValidRepr()
-      reads this
-    {
-      Repr == if bs == null then {this} else {this, bs}
+      && (valid? ==> off as nat + 4096 <= |fs.data[ino]|)
     }
 
     predicate {:opaque} ValidBytes()
       reads this, bs, fs
       requires fs.ValidDomains()
-      requires bs != null
     {
       && |bs.data| == 4096
       && off as nat + 4096 <= |fs.data[ino]|
@@ -51,12 +49,11 @@ module FileCursor {
     }
 
     predicate Valid()
-      reads this, Repr, fs.Repr, i.Repr
+      reads Repr(), fs.Repr, i.Repr
     {
-      && ValidRepr()
       && fs.ValidDomains()
       && ValidFs()
-      && (bs != null ==> ValidBytes())
+      && (valid? ==> ValidBytes())
     }
 
     // convenience function since this is a core concept
@@ -70,7 +67,7 @@ module FileCursor {
     predicate has_data(data: seq<byte>)
       reads this, bs
     {
-      bs != null && bs.data == data
+      valid? && bs.data == data
     }
 
     constructor(fs: TypedFilesys, ino: Ino, i: MemInode)
@@ -80,16 +77,17 @@ module FileCursor {
       ensures this.fs == fs
       ensures this.i == i
       ensures this.ino == ino
-      ensures fresh(Repr - {this})
-      ensures bs == null
+      ensures fresh(Repr())
+      ensures !valid?
     {
       this.ino := ino;
       this.i := i;
       this.fs := fs;
 
       this.off := 0;
-      this.bs := null;
-      this.Repr := {this};
+      var bs := NewBytes(0);
+      this.bs := bs;
+      this.valid? := false;
       new;
       reveal ValidFs();
       reveal ValidBytes();
@@ -97,7 +95,7 @@ module FileCursor {
 
     lemma data_ok()
       requires Valid()
-      requires bs != null
+      requires valid?
       ensures off as nat + 4096 <= |fs.data[ino]|
       ensures bs.data == fs.data[ino][off as nat .. off as nat + 4096]
     {
@@ -118,7 +116,7 @@ module FileCursor {
     twostate predicate buffer_fresh()
       reads this
     {
-      fresh(Repr - old(Repr))
+      fresh(Repr() - old(Repr()))
     }
 
     method advanceTo(txn: Txn, off': uint64)
@@ -128,29 +126,28 @@ module FileCursor {
       requires off' % 4096 == 0
       requires off' as nat < |fs.data[ino]|
       ensures this.off == off'
-      ensures bs != null
+      ensures valid?
       ensures buffer_fresh()
       ensures Valid()
     {
-      if off' == off && bs != null {
+      if off' == off && valid? {
         return;
       }
       reveal ValidFs();
       this.off := off';
       var blk := fs.readUnsafe(txn, ino, i, off, 4096);
       bs := blk;
-      Repr := {this, bs};
+      valid? := true;
       reveal ValidBytes();
     }
 
     method writeback(txn: Txn)
       returns (ok: bool)
       modifies ReprFs
-      requires ValidRepr()
       // note that ValidFs is preserved just by not modifying this directly and modifying bs
       requires ValidFs()
       requires fs.has_jrnl(txn)
-      requires bs != null && |bs.data| == 4096
+      requires valid? && |bs.data| == 4096
       ensures fs.types_unchanged()
       ensures buffer_fresh()
       ensures ok ==>
@@ -165,7 +162,7 @@ module FileCursor {
 
     method grow(txn: Txn)
       returns (ok: bool)
-      modifies Repr, ReprFs
+      modifies Repr(), ReprFs
       requires Valid()
       requires fs.has_jrnl(txn)
       requires |fs.data[ino]| + 4096 <= Inode.MAX_SZ
